\documentclass{article}
\usepackage[utf8]{inputenc}
\usepackage{amsmath}
\usepackage{amssymb}
\usepackage{graphicx}
\usepackage{graphics}
\usepackage{subfigure}
\usepackage{url}
\usepackage{flafter}
\usepackage{tikz}
\usepackage[american]{circuitikz}
\usepackage{pgfplots}


\begin{document}
\title{Lecture 16}
\maketitle

$\vec{B}=\vec{\nabla}\times\vec{A}$\\
$\vec{\nabla}.(\vec{\nabla}\times\vec{A})=0$\\
$x^{2}(l)+y^{2}(l)=R^{2}$\\
So, $x=R \cos \theta$\\
And $y=R\sin\theta$\\

$\vec{A}=\hat{e_{y}}\int_{x_{0}}^{x}B_{z}(x,y,z)dx+\hat{e_{z}}\left[\int_{y_{0}}^{y}B_{x}(x_{0},y,z)dy-\int_{x_{0}}^{x}B_{y}(x,y,z)dx\right] \neq \int\vec{B}\vec{dr}$\\

Now, we should prove that:
$\vec{\nabla}\vec{A}=\vec{B}$ , $\vec{B}=-B_{x}\hat{e_{x}}+B_{y}\hat{e_{y}}+B_{z}\hat{e_{z}}$\\

$(\vec{\nabla}\times \vec{A})=\frac{\partial A_{x}}{\partial z}.\frac{\partial A_{z}}{\partial x}=-\frac{\partial A_{z}}{\partial x}$\\

$\frac{\partial}{\partial x}\int_{x_{0}}^{x}B_{y}(x,y,z)dx=B_{y}(x,y,z)$\\

$(\vec{\nabla}\times\vec{A})_{z}=\frac{\partial A_{y}}{\partial x}-\frac{\partial A_{x}}{\partial y}=\frac{\partial A_{y}}{\partial x}$\\

$\frac{\partial}{\partial x}\int_{x_{0}}^{x}B_{z}(x,y,z)dx=B_{z}(x,y,z)$\\

\begin{align*}
(\vec{\nabla}\times\vec{A})_{x} &=\frac{\partial A_{z}}{\partial y}-\frac{\partial A_{y}}{\partial z}\\
&=\frac{\partial}{\partial y}\left[\int_{y_{0}}^{y}B_{x}(x,y,z)dy.\int_{x_{0}}^{x}B_{y}(x,y,z)dx\right]-\frac{\partial}{\partial z}\int_{x_{0}}^{x}B_{z}(x,y,z)dx\\
&= B_{x}(x_{0},y,z)-\int_{x_{0}}^{x}\left(\frac{B_{y}}{\partial y}+\frac{\partial B_{z}}{\partial z}\right)dx\\
\end{align*}
\newpage

$$\vec{\nabla}.\vec{B}=0 \rightarrow \mbox{So, } \frac{\partial B_{x}}{\partial x}=-\left(\frac{\partial B_{y}}{\partial y}+\frac{\partial B_{z}}{\partial z}\right)$$\\

$\frac{\partial}{\partial x}\int_{x_{0}}^{x}B_{y}(x,y,z)dx+\int_{x_{0}}^{x}B_{x}(x,y,z)dx=\int_{x_{0}}^{x}\frac{d}{dx}B_{x}(x,y,z)dx$\\

$\int_{x_{0}}^{x}dB_{x}(x,y,z)=B_{x}(x,y,z)-B_{x}(x_{0},y,z)$\\

If $\vec{\nabla}.\vec{B}=0$\\
$\vec{B}=\vec{\nabla}\vec{A}$\\
$\vec{A'}=\vec{A}+\vec{\nabla}\psi$\\
$\vec{\nabla}\times \vec{A'}=\vec{\nabla}\times
(\vec{\nabla}+\vec{\nabla}\psi)$\\
$\vec{\nabla}\times\vec{A'}=\vec{\nabla}\times\vec{A}=\vec{B}$\\
$\vec{\epsilon}=\vec{\nabla}(\varphi+c)$\\

\vspace{1cm}

\begin{align*} 
\vec{B} &=B_{z}\hat{e_{z}}\\
B_{z} &=constant\\
B_{x} &=B_{y}=0
\end{align*}

$\vec{A}=\hat{e_{y}}\int_{x=0}^{x}B_{z}(x,y,z)dx=\hat{e_{y}}B_{z}(x-x_{0})-\hat{e_{y}}B_{z}x-\hat{e_{y}}B_{z}x_{0}$\\

$\vec{\nabla}\times
(x B_{z}\hat{e_{y}})=B_{z}\hat{e_{3}}$\\

$\vec{A}=x B_{z}\hat{e_{y}}$ \hspace{1cm} $\vec{A}=-y B_{z}\hat{e_{x}}$\\

$$\vec{\nabla \times \vec{A'}}=\begin{vmatrix}
\hat{e_{x}} & \hat{e_{y}} & \hat{ee_{z}}\\
\frac{\partial}{\partial x} & \frac{\partial}{\partial y} & \frac{\partial}{\partial z}\\
=yB_{z} & 0 & 0
\end{vmatrix} = \frac{\partial}{\partial y}(yB_{z})\hat{e_{z}}=B_{z}\hat{e_{z}}$$\\

$\vec{A}\times
\vec{A'}=B_{z}(x\hat{e_{y}}+y\hat{e_{x}})=\vec{\nabla
}\psi$\\

$\psi=B_{z}xy$\\

$\vec{\nabla}\psi=\hat{e_{x}}\frac{\partial}{\partial x}(B_{z}xy)+\hat{e_{y}}\frac{\partial}{\partial y}(B_{z}xy)=yB_{z}\hat{e_{x}}+xB_{z}\hat{e_{y}}$\\

$\vec{A}=\frac{B_{z}}{2}(x\hat{e_{y}}-y\hat{e_{z}})$\\

$\vec{\nabla}.\epsilon=j/\epsilon_{0}$, $\vec{\nabla}.\vec{B}=0$, $\vec{\nabla}\times\vec{\epsilon}=-\frac{\partial\vec{B}}{\partial t}$, $\vec{\nabla}\times
\vec{B}=\mu_{0}\epsilon_{0}\frac{\partial \vec{\epsilon}}{\partial t}+\mu_{0}\vec{j}$\\

$\vec{\nabla}=q(\vec{\epsilon}+\vec{V}\times\vec{B})$\\

$\epsilon=-\vec{\nabla}\phi$ , \hspace{1cm} $\vec{B}=\vec{\nabla}\times\vec{A}$\\

$\vec{A'}= \vec{A}+\vec{\nabla}\psi$\\

$\vec{\nabla}.\vec{A'}=\lambda+\nabla \psi=0$\\

$\nabla\psi=-\lambda$,\hspace{1cm}, $\vec{\nabla}.\vec{A}=0$\\

$\vec{A'}=\vec{A}+\vec{\nabla}\lambda$\\
$\vec{\nabla}.\vec{A}=0$\\
$\vec{\nabla}\times \vec{A'}=0=\vec{\nabla}\vec{A}+\nabla\lambda$\\

 $\nabla \lambda=0$\hspace{1cm}, $\lambda=c$\\

$\vec{\nabla}\times \vec{\epsilon}=0$, $\vec{\epsilon}=-\vec{\nabla}\phi$\\

$\vec{\nabla}.\vec{B}=0$\\
$\vec{B}=\vec{\nabla}\times\vec{A}
$\\
$\vec{\nabla}\times\vec{\epsilon}=\frac{-\partial\vec{B}}{\partial t}$ \hspace{1cm} so$\vec{\nabla}\times
\vec{\epsilon\neq 0}$, $\vec{\epsilon}=-\vec{\nabla}\phi$\\

$\vec{\nabla}\times \vec{\epsilon}=-\frac{\partial\left(\vec{\nabla}\vec{A}\right)}{\partial t}$\\

$\vec{\nabla}\times
\left(\vec{\epsilon}+\frac{\partial\vec{A}}{\partial t}\right)=0$\\

$\vec{\epsilon+\frac{\partial\vec{A}}{\partial t}=-\vec{\nabla}}\phi$\\

$\epsilon=-\vec{\nabla}\phi=\frac{\partial\vec{A}}{\partial t}$, $\vec{B}=\vec{\nabla}\times\vec{A}$\\

$\vec{A'}=\vec{A}+\vec{\nabla}\psi(r,t)$\\

$\vec{B'}=\vec{\nabla}\times\vec{A'}=\vec{\nabla}\times \vec{A}=\vec{B}$\\

$\vec{E}=-\vec{\nabla}\phi-\frac{\partial A}{\partial t}-\frac{\partial}{\partial t}\nabla
\psi$\\

$\vec{B}=\vec{\nabla}\vec{A}$\\

$\vec{A'}=\vec{A}+\vec{\nabla}\psi$\\

$\vec{\epsilon=-\nabla\phi'-\frac{\partial A'}{\partial t}=\vec{\epsilon}}$\\

$\phi'=\phi-\frac{\partial \psi}{\partial t}$\\

$\vec{\epsilon'=-\vec{\nabla}}\phi'-\frac{\partial A'}{\partial t}$\\

$\vec{\nabla}.\epsilon=\rho/\epsilon_{0}$\\

$\vec{\nabla}\left(-\nabla\phi-\frac{\partial A}{\partial t}\right)=\rho/\epsilon_{0}$\\

$-\nabla^{2}\phi.\frac{\partial}{\partial t}\vec{\nabla}.\vec{A}=\rho/\epsilon_{0}$\\

$\nabla^{2}\phi=-\frac{\rho(\vec{r})}{\epsilon_{0}}$\\

$\phi(\vec{r})=\frac{1}{\epsilon_{0}\pi}\int\frac{\rho(\vec{r})dv'}{|\vec{r}-\vec{r'}|}$\\

$\nabla^{2}\phi-\frac{1}{c^{2}}\frac{\partial^{2}\phi}{\partial t^{2}}=\rho/\epsilon_{0}$\\

$\vec{\nabla}.\vec{A}+\frac{1}{c^{2}}\frac{\partial
\phi}{\partial t}=0$


\end{document}