\documentclass{article}
\usepackage{amsmath, amssymb}
\begin{document}
\begin{equation*}
 \hspace*{-19.5cm}         \boldsymbol{A}=a_{ij}
\end{equation*}
\begin{equation*}
\hspace*{-12cm}  det(A)=\sum_{j=1}^{n} a_{ij}\times(-1)^{i+j}\times M_{ij}\;\;\;\;\;M_{ij}=nun\;\;\;of\;\;\;\ \boldsymbol{a_{ij}}
\end{equation*}
\begin{equation*}
\hspace{-10.5cm} D_{n}=\begin{bmatrix}
a_{11}&a_{12}&\cdots&a_{1n}\\
a_{21}&a_{22}&\cdots&a_{2n}\\
\vdots&\vdots&\ddots&\vdots\\
a_{n1}&a_{n2}&\cdots&a_{nn}
\end{bmatrix}=\sum_{i_{1}i_{2}\cdots i_{n}}^{n} \epsilon_{i_{1}i_{2}\cdots i_{n}}
\;\;\;\;\;\;\;\;\;a_{1i_{1}}a_{2i_{2}}\cdots a_{ni_{n}}
\end{equation*}
\begin{equation*}
\hspace{-9.1cm}  D_{2}= \begin{bmatrix}
a_{11}a_{12}\\
a_{21}a_{22}
\end{bmatrix}
=\sum_{i=1}^{2} \sum_{j=1}^{2} \epsilon_{ij} a_{1i} a_{2j}
=\epsilon_{12} a_{11} a_{22} + \epsilon_{21} a_{12} a_{21}
=a_{11} a_{22} - a_{12} a_{21}
\end{equation*}
\begin{equation*}
\hspace{-18.6cm} \boldsymbol{ D_n\Rightarrow k*D_n}
\end{equation*}
\begin{equation*}
\hspace{-16cm} \begin{bmatrix}
k*a_{11}&k*a_{12}&\cdots&k*a_{1n}\\
k*a_{21}&k*a_{22}&\cdots&k*a_{2n}\\
\vdots&\vdots&\ddots&\vdots\\
k*a_{n1}&k*a_{n2}&\cdots&k*a_{nn}
\end{bmatrix}
\end{equation*}
\begin{equation*}
\hspace{-10.5cm} \begin{bmatrix}
Ca_{11}+Kb_{1}a_{12}a_{13}\\
Ca_{21}+Kb_{2}a_{22}a_{23}\\
Ca_{31}+Kb_{3}a_{32}a_{33}
\end{bmatrix}=C\times \begin{bmatrix}
a_{11}&a_{12}&a_{13}\\
a_{21}&a_{22}&a_{23}\\
a_{31}&a_{32}&a_{33}
\end{bmatrix} + K\times \begin{bmatrix}
b_{!}&a_{12}&a_{13}\\
b_{2}&a_{22}&a_{23}\\
b_{3}&a_{32}&a_{33}
\end{bmatrix}
\end{equation*}
\begin{eqnarray*}
\sum_{i,j=1}^{n} S_{ij} A_{ij}&=&0\\
&=&\sum_{i,j=1}^{n} S_{ji} A_{ji}\\
&=&-\sum_{i,j=1}^{n} S_{ij} A_{ij}
\end{eqnarray*}

$$\hspace{-15cm} \boldsymbol{Linear System  \;of Equations:}$$
\begin{equation*}
a_{1}x_{!}+a_{2}x_{2}+a_{3}x_{3}=h_{1}
\end{equation*}
\begin{equation*}
b_{1}x_{1}+b_{2}x_{2}+b_{3}x_{3}=h_{2}
\end{equation*}
\begin{equation*}
c_{1}x_{1}+c_{2}x_{2}+c_{3}x_{3}=h_{3}
\end{equation*}
\begin{equation*}
\hspace{1cm} \begin{bmatrix}
a_{!}&a_{2}&a_{3}\\
b_{1}&b_{2}&b_{3}\\
c_{1}&c_{2}&c_{3}
\end{bmatrix}
\end{equation*}
\begin{equation*}
x_{1}*D=\begin{bmatrix}
x_{!}a_{1}&a_{2}&a_{3}\\
x_{1}b_{1}&b_{2}&b_{3}\\
x_{1}c_{1}&c_{2}&c_{3}
\end{bmatrix}
\end{equation*}
\begin{equation*}
x_{1}=(\frac{1}{D})*\begin{bmatrix}
h_{1}&a_{2}&a_{3}\\
h_{2}&b_{2}&b_{3}\\
h_{3}&c_{2}&c_{3}
\end{bmatrix}
\end{equation*}



\end{document}