\documentclass[11]{article}
\usepackage[utf8]{inputenc}
\usepackage{amsmath}
\usepackage{amssymb}
\usepackage{graphicx}
\usepackage{graphics}
\usepackage{subfigure}
\usepackage{url}
\usepackage{flafter}

\usepackage{tikz}
\usepackage[american]{circuitikz}
\usepackage{pgfplots}
\usepackage{hyperref}


\begin{document}

\begin{titlepage}
\begin{center}
\Large\textbf{Lecture.8}
\end{center}

\begin{itemize}
\item Scalar Triple Product\\
\vspace{0.3cm}

$
\vec{A}.(\vec{B}\times \vec{C})
$

\item Reciprocal Lattice\\

$a= Lattice Spacing $
\begin{center}
\includegraphics[scale=0.5]{1.png}

\end{center}

\begin{equation*}
\large
\scalebox{1.5}{$\frac{\hbar}{2m} \frac{d^{2}\psi(x)}{dx^{2}}+V(x)\psi=\epsilon \psi$}
\end{equation*}
\vspace{1cm}

$\psi (x) \rightarrow \psi (x+a)$\\

$x \rightarrow (x+a) = y \rightarrow x=y-a$



\begin{equation*}
\begin{split}
V(x+a)& =V(a)\\
& =\frac{\hbar^{2}}{2} \frac{d^{2}\psi(x+a)}{d(x+a)^{2}}+V(x+a) \psi(x+a)\\
& =\epsilon \psi(x+a)
\end{split}
\end{equation*}

$\psi(x+na), \hspace{5mm}  n \in \mathbb{z}$\\

$\int |\psi|^{2} dx = 1$\\

$\psi (x+na)= \lambda \psi(x)$\\

$|\psi (x+na)|^{2} = |\lambda^{2}| |\psi (x)|^{2}$\\

$ so, |\lambda|^{2} =1 \rightarrow \lambda =e^{i \theta} \hspace{5mm}, \theta=0$\\

\begin{equation*}
\large
\scalebox{1.5}{-$ \frac{\hslash^{2}}{2m} \frac{d^{2} \psi}{dx^{2}} + V(x) \psi = \epsilon \psi(x)$}
\end{equation*}

\begin{align*}
\psi (x) & = e^{i p_{x}} U_{p}(x)  &  e^{i(p+a} U_{p}(x+a)\\
U_{p}(x+a) & = U_{p}(x) &  & =e^{ipx} U_{p}(x)\\
\psi(x+a) & = \psi(x)   & e^{ipx} & =1\\
so, p & = \frac{2 \pi n}{a}\\
If, \hspace{1cm} e^{2 i \pi p a} & =1\\
Then, p=\frac{n}{a} \hspace{0.5cm} ,n \in \gamma
\end{align*}

\item 1D

\begin{align*}
\vec{R} & =na \hat{i}\\
& =n \vec{a}\\
a & =a \hat{i} (Lattice Vector)\\
P(momentum) & =n \vec{a} \hspace{0.5cm} \vec{a'} = \frac{1}{a} \hat{i}
\end{align*}

\item 3D

\begin{equation*}
\begin{split}
\vec{R} & = 2 \vec{a}+2 \vec{b}\\
& =2a \hat{i}+2b \hat{j}\\
\vec{R} & =n_{a} \vec{a}+n_{b} \vec{b}+n_{c} \vec{c}\\
\vec{a}, \vec{b}, \vec{c} \hspace{3mm} \mbox{are the basis of the crystal lattice}
\end{split}
\end{equation*}
 
 \begin{center}
 \includegraphics[scale=0.5]{2.png}
 \end{center}
$\psi(x)=e^{i \vec{p} . \vec{r}} \hspace{2mm} \mbox{must be invariant under any lattice transformatin}$

$\psi(\vec{r}+ \vec{R})= \psi( \vec{r}) \rightarrow e^{i 2 \pi \vec{p}. \vec{r}} \times e^{i 2 \pi \vec{p}. \vec{r}}$\\

$e^{i 2 \pi \vec{p}. \vec{r}}=1$\\

$ \vec{p}=p_{1} \vec{a'}+p_{2} \vec{b'}+p_{3} \vec{c'}$\\

assume that $ \vec{R}= \vec{a}$
$e^{i 2 \pi \vec{p}. \vec{r}}$\\

so $ \vec{p}=\frac{na'}{a}=n'_{a} \vec{a'}$\\

$ \vec{R}= \vec{h} \rightarrow e^{i 2 \pi \vec{p}. \vec{h}}=1$\\

SO. $ \vec{P}=\frac{n'_{h}}{h}=n_{h} \vec{h''}$\\

 $ \vec{R}= \vec{c} \rightarrow e^{i 2 \pi \vec{p}. \vec{c}}=1$\\
 
 so, $ \vec{p}= \frac{n'_{c}}{c}=n'_{c} \vec{c'}$\\
 
 $\vec{p}=n'_{a} \vec{a'}+n'_{h} \vec{h'}+n_{c} \vec{c'}$\\
 
$\vec{p}. \vec{a}= n_{a}$\\ 
 
 \begin{align*}
\vec{a'}.\vec{a} & =1  & \vec{a'}.\vec{h} & =0 & \vec{a'}.\vec{c} & =0\\
\vec{h'}.\vec{h} & =1 & \vec{h'}.\vec{a} & =0 & \vec{h'}.\vec{c} & =0\\
\vec{c'}.\vec{c} & =1 & \vec{c'}.\vec{a} & =0 & \vec{c'}.\vec{h} & =0
 \end{align*}
 
 \newpage
 \begin{center}
 \begin{eqnarray*}
& \vec{h'} \alpha (\vec{a} \times \vec{c})\\
& \mbox{So,} \vec{h'}= \lambda ( \vec{a} \times \vec{c})\\
& \vec{h'}. \vec{h}= \lambda ( \vec{a} \times \vec{c}). \vec{h} =1\\
& \mbox{So, } \vec{h'}=\lambda ( \vec{a} \times \vec{c}). \vec{h} \hspace{3mm} \lambda =\frac{1}{(\vec{a} \times \vec{c}). \vec{h}}\\
& \mbox{So,} \vec{h'}=\frac{\vec{a} \times \vec{c}}{(\vec{a} \times \vec{c}). \vec{h}} 
 \end{eqnarray*}
 \end{center}
 
 $ \vec{c'} =\frac{(\vec{a} \times \vec{h})}{(\vec{a} \times \vec{h}. \vec{c}}$\\
 
 $ \vec{a'}=\frac{(\vec{h} \times \vec{c})}{(\vec{h} \times \vec{c}. \vec{a})}
$\\

\item 
$\vec{A} \times (\vec{B} \times \vec{C}) \neq (\vec{A} \times \vec{B}) \times \vec{C} $

$(\hat{e_{1}} \times \hat{e_{1}}) \times \hat{e_{2}}=0$\\

$\hat{e_{1}} \times (\hat{e_{1}} \times \hat{e_{2}})=\hat{e_{1}} \times \hat{e_{3}}=-\hat{e_{2}}$\\

\item $\vec{A} \times (\vec{B} \times \vec{C})=\vec{B}(\vec{A}.\vec{C})-\vec{C}(\vec{A}.\vec{B})$

$(\vec{B}\times \vec{C})_{k} = \sum_{pq} \epsilon_{kpq} B_{p} C_{q}$\\

$c_{i}= \sum_{jk} \epsilon_{ijk} A_{j} B_{k}$\\

$(\vec{A} \times (\vec{B} \times \vec{C}))_{i} = \sum_{jk} \epsilon_{ijk} A_{j} \epsilon_{kpq} B_{p}C_{q}$\\

\begin{align*}
\sum_{i} \hat{e_{i}}(\vec{A} \times (\vec{B} \times \vec{C}))_{i} & =\sum_{i} \hat{e_{i}} \sum_{jk} A_{j} \sum_{pq} \epsilon_{kpq} B_{p} C_{q}\\
& =\sum_{ij} \sum_{pq} \hat{e_{i}} A_{j} B_{p} C_{q} \sum_{k} \epsilon_{ijk} \epsilon_{kpq}\\
\sum_{k} \epsilon_{ijk} \epsilon{kpq} & =\sum_{k} \epsilon_{kij} \epsilon_{kpq} &=\delta_{ip} \delta_{jq}-\delta_{ip} \delta_{jp}\\
& =\sum_{i} \hat{e_{i}} B_{i} \sum_{j} A_{j} C_{j}-\sum_{i} \hat{e_{i}} C_{i} \sum_{j} A_{j} B_{j}\\
& =\vec{B}(\vec{A}. \vec{C})- \vec{c}(\vec{A}.\vec{B})
\end{align*}





 
 

\end{itemize}

\end{titlepage}

\end{document}